# 对数函数

## 和公式
$$
\begin{aligned}
    \log_a{b} + \log_a{c} = \log_a{bc}
\end{aligned}
$$

推导过程：
$$
\begin{aligned}
    & \because bc = a^{ \log_a{b} } a^{ \log_a{c} } = a^{ \log_a{b} + \log_a{c} }\\
    & \therefore \log_a{bc} = \log_{a}{a^{ \log_a{b} + \log_a{c} }} =\log_a{b} + \log_a{c}
\end{aligned}
$$


## 差公式
$$
\begin{aligned}
    \log_a{b} - \log_a{c} = \log_a{\frac{b}{c}}
\end{aligned}
$$

推导过程：
$$
\begin{aligned}
    & \because \frac{b}{c} = \frac{a^{\log_{a}{b}}}{a^{\log_{a}{c}}} = a^{\log_{a}{b} - \log_{a}{c}} \\
    & \therefore \log_{a}{\frac{b}{c}} = \log_{a}{a^{\log_{a}{b} - \log_{a}{c}}} = \log_{a}{b} - \log_{a}{c}
\end{aligned}
$$


## 换底公式
$$
\begin{aligned}
    \log_a{b} = \frac{ \log_c{b} }{ \log_c{a} }
\end{aligned} \\
$$
推导过程：

$$ 
\begin{aligned}
& \because \log_{c}{a} = \log_{c}{b^{ \log_{b}{a} }} 
= \log_{b}{a} \log_{c}{b} \\
& \therefore \log_{b}{a} = \frac{ \log_{c}{a} }{ \log_{a}{b} }
\end{aligned}
$$


## 不知道是什么公式
$$ 
\log_{a}{b} = \frac{ \log_{a}{c} }{ \log_{b}{c} }
$$

推导过程：
$$
\begin{aligned}
    & \because \log_{a}{c} = \log_{a}{b^{ \log_{b}{c} }} = \log_{b}{c} \log_{a}{b} \\
    & \therefore \log_{a}{b} = \frac{ \log_{a}{c} }{ \log_{b}{c} }
\end{aligned}
$$


## 真底互换公式
$$
\begin{aligned}
    \log_{a}{b} = \frac{1}{ \log_{b}{a} }
\end{aligned}
$$

推导过程：

将上一个公式中的 $c$ 替换为 $a$ 即可得到：
$$
\begin{aligned}
    & \because a = b^{ \log_{b}{a} } \\
    & \therefore \log_{a}{a} = \log_{a}{b^{ \log_{b}{a} }} = \log_{b}{a} \log_{a}{b} = 1 \\
    & \therefore \log_{a}{b} = \frac{1}{ \log_{b}{a} }
\end{aligned}
$$